Move BAT files to examples directory

examples/bat/BAT.v
@@ -1,7 +1,6 @@
 (** * Basic Attention Token contract *)
-(** This implementation of the Basic Attention Token is a based on
-    https://github.com/brave-intl/basic-attention-token-crowdsale/blob/66c886cc4bfb0493d9e7980f392ca7921ef1e7fc/contracts/BAToken.sol
-    The implementation includes some minor changes that fixes bugs present in the original Solidity implementation.
+(** Implementation of the Basic Attention Token.
+    Ported from https://github.com/brave-intl/basic-attention-token-crowdsale/blob/66c886cc4bfb0493d9e7980f392ca7921ef1e7fc/contracts/BAToken.sol
 
     This file contains contract function definitions and proofs.
     All contract types and utility functions are defined in [ConCert.Execution.Examples.BATCommon].
@@ -11,7 +10,6 @@
 *)
 From Coq Require Import Lia.
 From Coq Require Import List.
-From Coq Require Import Morphisms.
 From Coq Require Import ZArith.
 From ConCert.Utils Require Import Automation.
 From ConCert.Utils Require Import RecordUpdate.
@@ -21,16 +19,15 @@ From ConCert.Execution Require Import Containers.
 From ConCert.Execution Require Import Extras.
 From ConCert.Execution Require Import Monads.
 From ConCert.Execution Require Import Serializable.
-From ConCert.Execution.Examples Require Import BATCommon.
-From ConCert.Execution.Examples Require Import Common.
-From ConCert.Execution.Examples Require EIP20Token.
+From ConCert.Execution Require Import Common.
+From ConCert.Examples.BAT Require Import BATCommon.
+From ConCert.Examples.EIP20 Require EIP20Token.
 Import RecordSetNotations.
 Import ListNotations.
 
 
-
 (** * Contract functions *)
-Section BATFixed.
+Section BAT.
 Context {BaseTypes : ChainBase}.
 
 Open Scope N_scope.
@@ -41,25 +38,6 @@ Open Scope N_scope.
 Definition init (chain : Chain)
                 (ctx : ContractCallContext)
                 (setup : Setup) : option State :=
-  (** BAToken should not be deployable if one of the following conditions does not hold on [setup]
-      - funding period is non empty
-      - funding period does not start before the slot where the contract is deployed
-      - minimum tokens to fund should not be less than the maximum tokens allowed
-      - the initial supply of tokens should be less than the maximum tokens allowed
-      - token exchange rate must be larger than 0
-      - it must be possible to get over minimum token bound without going over maximum
-      For the last condition we check that [tokenExchangeRate <= tokenCreationCap - tokenCreationMin], however this does exclude
-      a few possible configurations where the contract still works as intended, however these are not likely to
-      come up in real usecases.
-  *)
-  do _ <- throwIf ((setup.(_fundingEnd) <=? setup.(_fundingStart))%nat
-          || (setup.(_fundingStart) <? chain.(current_slot))%nat
-          || (setup.(_tokenCreationCap) <? setup.(_tokenCreationMin))
-          || (setup.(_tokenCreationCap) <? setup.(_batFund))
-          || (setup.(_tokenExchangeRate) =? 0)
-          || ((setup.(_tokenCreationCap) - setup.(_tokenCreationMin)) <? setup.(_tokenExchangeRate))
-          || address_eqb setup.(_batFundDeposit) ctx.(ctx_contract_address)
-          || address_eqb setup.(_fundDeposit) ctx.(ctx_contract_address)) ;
   let token_state := {|
       EIP20Token.balances := FMap.add setup.(_batFundDeposit) setup.(_batFund) FMap.empty;
       EIP20Token.total_supply := setup.(_batFund);
@@ -83,11 +61,10 @@ Definition init (chain : Chain)
 (** ** Create Tokens *)
 (** This entrypoint allows users to fund the crowdsale in return for tokens *)
 Definition try_create_tokens sender (sender_payload : Amount) current_slot state :=
- (** Early return if funding is finalized, funding period hasn't started yet, or funding period is over *)
+ (* early return if funding is finalized, funding period hasn't started yet, or funding period is over *)
   do _ <- throwIf (state.(isFinalized)
           || (Nat.ltb current_slot state.(fundingStart))
-          || (Nat.ltb state.(fundingEnd) current_slot)
-          || (address_eqb sender state.(batFundDeposit))) ;
+          || (Nat.ltb state.(fundingEnd) current_slot)) ;
   (** Here we deviate slightly from the reference implementation. They only check for = 0,
       but since ConCert's payloads may be negative numbers, we must extend this check to <= 0 *)
   do _ <- throwIf (Z.leb sender_payload 0) ;
@@ -171,16 +148,14 @@ Definition receive_bat (chain : Chain)
 Close Scope Z_scope.
 
 (** Composes EIP20Token.receive and receive_bat by first executing EIP20Token.receive (if the message is an EIP20 message),
-    and otherwise executes receive_bat *)
+   and otherwise executes receive_bat *)
 Definition receive (chain : Chain)
                     (ctx : ContractCallContext)
                    (state : State)
                    (maybe_msg : option Msg)
                    : option (State * list ActionBody) :=
   match maybe_msg with
-  | Some (tokenMsg msg) =>
-                     do _ <- throwIf (negb (isFinalized state)) ;
-                     do res <- EIP20Token.receive chain ctx state.(token_state) (Some msg) ;
+  | Some (tokenMsg msg) => do res <- EIP20Token.receive chain ctx state.(token_state) (Some msg) ;
                      let new_state := state<|token_state := fst res|> in
                          Some (new_state, snd res)
   | _ => receive_bat chain ctx state maybe_msg
@@ -189,11 +164,9 @@ Definition receive (chain : Chain)
 Definition contract : Contract Setup Msg State :=
   build_contract init receive.
 
-
-
 (** * Contract properties *)
 Section Theories.
-(* begin hide *)
+(* begind hide *)
 (* Tactics to simplify proof steps *)
 Tactic Notation "contract_simpl" := contract_simpl receive init.
 
@@ -256,14 +229,12 @@ Proof.
 Qed.
 
 Lemma try_transfer_is_some : forall state chain ctx to amount,
-  (isFinalized state) = true ->
   (ctx_amount ctx <= 0)%Z /\
   amount <= with_default 0 (FMap.find (ctx_from ctx) (balances state))
     <-> isSome (receive chain ctx state (Some (transfer to amount))) = true.
 Proof.
-  intros * finalized.
+  intros.
   unfold balances. cbn.
-  rewrite finalized. cbn.
   destruct_match eqn:receive;
     now erewrite EIP20Token.try_transfer_is_some, receive.
 Qed.
@@ -306,7 +277,7 @@ Lemma try_transfer_from_preserves_other_allowances : forall prev_state new_state
     forall account, account <> from ->
       FMap.find account (allowances prev_state) = FMap.find account (allowances new_state).
 Proof.
-  intros * receive_some account account_not_from.
+  intros * receive_some.
   contract_simpl.
   eapply EIP20Token.try_transfer_from_preserves_other_allowances; eauto.
 Qed.
@@ -316,7 +287,7 @@ Lemma try_transfer_from_preserves_other_allowance : forall prev_state new_state 
     forall account, account <> (ctx_from ctx) ->
       get_allowance (token_state prev_state) from account = get_allowance (token_state new_state) from account.
 Proof.
-  intros * receive_some account account_not_sender.
+  intros * receive_some.
   contract_simpl.
   eapply EIP20Token.try_transfer_from_preserves_other_allowance; eauto.
 Qed.
@@ -324,16 +295,14 @@ Qed.
 Lemma try_transfer_from_is_some : forall state chain ctx from to amount,
   let get_allowance_ account := FMap.find account (with_default (@FMap.empty (FMap Address TokenValue) _) (FMap.find from (allowances state))) in
   (ctx_amount ctx >? 0)%Z = false ->
-  (isFinalized state) = true ->
   isSome (FMap.find from (allowances state)) = true
   /\ isSome (get_allowance_ (ctx_from ctx)) = true
   /\ amount <= with_default 0 (FMap.find from (balances state))
   /\ amount <= with_default 0 (get_allowance_ (ctx_from ctx))
     <-> isSome (receive chain ctx state (Some (transfer_from from to amount))) = true.
 Proof.
-  intros * sender_amount_zero finalized.
+  intros * amount_zero.
   unfold balances, allowances, get_allowance_. cbn.
-  rewrite finalized. cbn.
   destruct_match eqn:receive;
     now erewrite EIP20Token.try_transfer_from_is_some, receive.
 Qed.
@@ -374,7 +343,7 @@ Lemma try_approve_preserves_other_allowances : forall prev_state new_state chain
     forall account, account <> (ctx_from ctx) ->
       FMap.find account (allowances prev_state) = FMap.find account (allowances new_state).
 Proof.
-  intros * receive_some account account_not_sender.
+  intros * receive_some.
   contract_simpl.
   eapply EIP20Token.try_approve_preserves_other_allowances; eauto.
 Qed.
@@ -384,29 +353,18 @@ Lemma try_approve_preserves_other_allowance : forall prev_state new_state chain 
     forall account, account <> delegate ->
       get_allowance (token_state prev_state) (ctx_from ctx) account = get_allowance (token_state new_state) (ctx_from ctx) account.
 Proof.
-  intros * receive_some account account_not_delegate.
+  intros * receive_some.
   contract_simpl.
   eapply EIP20Token.try_approve_preserves_other_allowance; eauto.
 Qed.
 
 Lemma try_approve_is_some : forall state chain ctx delegate amount,
-  (ctx_amount ctx >? 0)%Z = false /\ (isFinalized state) = true <-> isSome (receive chain ctx state (Some (approve delegate amount))) = true.
+  (ctx_amount ctx >? 0)%Z = false <-> isSome (receive chain ctx state (Some (approve delegate amount))) = true.
 Proof.
   intros.
   cbn.
-  destruct_match eqn:finalized_check;
-    destruct_throw_if finalized_check; split.
-  - intros (sender_amount_zero & finalized).
-    destruct_match eqn:receive.
-    + reflexivity.
-    + now erewrite EIP20Token.try_approve_is_some, receive in sender_amount_zero.
-  - destruct_match eqn:receive; try discriminate.
-    split.
-    + now erewrite EIP20Token.try_approve_is_some, receive.
-    + now rewrite Bool.negb_false_iff in finalized_check.
-  - intros (sender_amount_zero & finalized).
-    now rewrite finalized in finalized_check.
-  - discriminate.
+  destruct_match eqn:receive;
+    now erewrite EIP20Token.try_approve_is_some, receive.
 Qed.
 
 
@@ -507,7 +465,6 @@ Lemma try_create_tokens_is_some : forall state chain ctx,
   /\ ((fundingStart state) <= (current_slot chain))%nat
   /\ ((current_slot chain) <= (fundingEnd state))%nat
   /\ (total_supply state) + ((Z.to_N (ctx_amount ctx)) * (tokenExchangeRate state)) <= (tokenCreationCap state)
-  /\ (ctx_from ctx) <> (batFundDeposit state)
     <-> exists x y, receive chain ctx state (Some create_tokens) = Some (x, y).
 Proof.
   split;
@@ -516,8 +473,7 @@ Proof.
     contract_simpl;
     autorewrite with BoolElim in *;
     destruct_or_hyps;
-    try easy;
-    now destruct_address_eq.
+    try easy.
 Qed.
 
 Lemma try_create_tokens_acts_correct : forall prev_state new_state chain ctx new_acts,
@@ -696,7 +652,7 @@ Lemma init_other_balances_correct : forall state chain ctx setup,
     forall account, account <> state.(batFundDeposit) ->
     with_default 0 (FMap.find account (balances state)) = 0.
 Proof.
-  intros * init_some account account_not_batfund.
+  intros * init_some account account_not_funddeposit.
   contract_simpl.
   now setoid_rewrite FMap.find_add_ne.
 Qed.
@@ -742,7 +698,7 @@ Qed.
 
 
 
-(** ** EIP20 functions preserve sum of balances *)
+(** ** Functions preserve sum of balances *)
 
 Lemma try_transfer_preserves_balances_sum : forall prev_state new_state chain ctx to amount new_acts,
   receive chain ctx prev_state (Some (transfer to amount)) = Some (new_state, new_acts) ->
@@ -777,8 +733,7 @@ Lemma try_create_tokens_update_balances_sum : forall prev_state new_state chain 
 Proof.
   intros * receive_some.
   contract_simpl.
-  unfold EIP20Token.sum_balances.
-  cbn in *.
+  unfold EIP20Token.sum_balances. cbn in *.
   setoid_rewrite EIP20Token.add_is_partial_alter_plus; auto.
   destruct (FMap.find (ctx_from ctx) (balances prev_state)) eqn:from_balance.
   - setoid_rewrite from_balance.
@@ -821,39 +776,6 @@ Proof.
   setoid_rewrite FMap.elements_add; auto.
   rewrite fin_maps.map_to_list_empty.
   now apply N.add_0_r.
-Qed.
-
-
-
-(** ** Init validation *)
-
-Lemma deployed_implies_constants_valid bstate caddr :
-  reachable bstate ->
-  env_contracts bstate caddr = Some (contract : WeakContract) ->
-  exists cstate,
-    contract_state bstate caddr = Some cstate
-    /\ (cstate.(fundingStart) < cstate.(fundingEnd))%nat
-    /\ cstate.(tokenCreationMin) <= cstate.(tokenCreationCap)
-    /\ cstate.(initSupply) <= cstate.(tokenCreationCap)
-    /\ cstate.(tokenExchangeRate) <> 0
-    /\ cstate.(tokenExchangeRate) <= cstate.(tokenCreationCap) - cstate.(tokenCreationMin)
-    /\ cstate.(batFundDeposit) <> caddr
-    /\ cstate.(fundDeposit) <> caddr.
-Proof.
-  contract_induction; intros; auto.
-  - contract_simpl. cbn.
-    autorewrite with BoolElim in *.
-    now destruct_address_eq.
-  - destruct_message;
-    now contract_simpl.
-  - destruct_message;
-    now contract_simpl.
-  - instantiate (AddBlockFacts := fun _ _ _ _ _ _ => True).
-    instantiate (DeployFacts := fun _ _ => True).
-    instantiate (CallFacts := fun _ _ _ _ => True).
-    unset_all; subst; cbn in *.
-    destruct_chain_step; auto.
-    destruct_action_eval; auto.
 Qed.
 
 
@@ -950,8 +872,7 @@ Lemma constants_are_constant bstate caddr (trace : ChainTrace empty_state bstate
       /\ cstate.(tokenCreationMin) = setup.(_tokenCreationMin)
       /\ cstate.(initSupply) = setup.(_batFund).
 Proof.
-  apply (lift_dep_info_contract_state_prop contract);
-    intros *; clear trace bstate caddr.
+  apply (lift_dep_info_contract_state_prop contract); intros *.
   - intros init_some.
     now apply init_constants_correct in init_some.
   - intros IH receive_some.
@@ -1022,7 +943,7 @@ Lemma can_finalize_if_creation_min : forall bstate (reward : Amount) (caddr crea
   reachable bstate ->
   emptyable (chain_state_queue bstate) ->
   (exists cstate,
-    env_contracts bstate caddr = Some (BATFixed.contract : WeakContract)
+    env_contracts bstate caddr = Some (BAT.contract : WeakContract)
     /\ env_contract_states bstate caddr = Some (serializeState cstate)
     /\ (tokenCreationMin cstate) <= (total_supply cstate)
     /\ address_is_contract (fundDeposit cstate) = false)
@@ -1030,7 +951,7 @@ Lemma can_finalize_if_creation_min : forall bstate (reward : Amount) (caddr crea
       exists bstate', reachable_through bstate bstate'
         /\ emptyable (chain_state_queue bstate')
         /\ exists cstate',
-        env_contracts bstate' caddr = Some (BATFixed.contract : WeakContract)
+        env_contracts bstate' caddr = Some (BAT.contract : WeakContract)
         /\ env_contract_states bstate' caddr = Some (serializeState cstate')
         /\ (isFinalized cstate') = true.
 Proof.
@@ -1054,10 +975,11 @@ Proof.
       (prev_state' & msg' & new_state' & serialize_prev_state & _ & serialize_new_state & receive_some).
     setoid_rewrite deserialize_serialize in serialize_prev_state.
     inversion serialize_prev_state. subst.
+    clear serialize_prev_state.
     apply receive_total_supply_increasing in receive_some as total_supply_increasing; try (cbn; lia).
     apply receive_preserves_constants in receive_some as (? & ? & ? & ? & ? & ? & ? & ?).
     repeat match goal with
-    | H : _ prev_state' =  _ new_state' |- _=> rewrite H in *; clear H
+    | H : _ prev_state' =  _ new_state' |- _=> try rewrite H in *; clear H
     end.
     exists new_state'.
     rewrite_environment_equiv; cbn; repeat split; eauto;
@@ -1084,7 +1006,7 @@ Proof.
 
     (* We can now evaluate the action we added giving us a ChainState where
         the token is in its finalized state *)
-    evaluate_action BATFixed.contract; try easy.
+    evaluate_action BAT.contract; try easy.
     + (* Prove that there is enough balance to evaluate action *)
       now apply account_balance_nonnegative.
     + (* Prove that receive action returns Some *)
@@ -1092,7 +1014,7 @@ Proof.
       * specialize try_finalize_isFinalized_correct as [_ finalized_new_cstate]; eauto.
         now erewrite <- (try_finalize_only_change_isFinalized _ _ _ _ _ receive_some),
                      finalized_new_cstate, (try_finalize_acts_correct _ _ _ _ _ receive_some) in receive_some.
-      * easy.
+      * repeat split; eauto.
     + cbn in *.
       clear contract_state slot_hit creation_min.
       update_all;
@@ -1125,19 +1047,20 @@ Lemma can_finalize_if_deployed : forall deployed_bstate (reward : Amount) (caddr
   NoDup accounts ->
   Forall (fun acc => address_is_contract acc = false) accounts ->
   (exists deployed_cstate,
-    env_contracts deployed_bstate caddr = Some (BATFixed.contract : WeakContract)
+    env_contracts deployed_bstate caddr = Some (BAT.contract : WeakContract)
     /\ env_contract_states deployed_bstate caddr = Some (serializeState deployed_cstate)
     /\ (((tokenCreationMin deployed_cstate) - (total_supply deployed_cstate))) <=
             ((Z.to_N (spendable_balance deployed_bstate accounts)) * (tokenExchangeRate deployed_cstate))
+    /\ deployed_cstate.(tokenExchangeRate) <= deployed_cstate.(tokenCreationCap) - deployed_cstate.(tokenCreationMin)
     /\ ((fundingStart deployed_cstate) <= (current_slot (env_chain deployed_bstate)))%nat
     /\ ((current_slot (env_chain deployed_bstate)) < (fundingEnd deployed_cstate))%nat
     /\ address_is_contract (fundDeposit deployed_cstate) = false
-    /\ ~ In (batFundDeposit deployed_cstate) accounts)
+    /\ deployed_cstate.(tokenExchangeRate) <> 0)
       ->
       exists bstate, reachable_through deployed_bstate bstate
         /\ emptyable (chain_state_queue bstate)
         /\ exists cstate,
-        env_contracts bstate caddr = Some (BATFixed.contract : WeakContract)
+        env_contracts bstate caddr = Some (BAT.contract : WeakContract)
         /\ env_contract_states bstate caddr = Some (serializeState cstate)
         /\ (isFinalized cstate) = true.
 Proof.
@@ -1145,8 +1068,8 @@ Proof.
   (* Empty the action queue so that we can add new blocks *)
   empty_queue H; destruct H as
     (cstate & contract_deployed & contract_state & enough_balance_to_fund &
-     funding_period_started & funding_period_not_over &
-     fund_deposit_not_contract & bat_fund_not_in_accounts);
+     can_hit_fund_min & funding_period_started & funding_period_not_over &
+     fund_deposit_not_contract & echange_rate_nonzero);
     (* Prove that H is preserved after transfers, discarding invalid actions, calling other contracts and deploying contracts *)
     only 3: destruct (address_eqdec caddr to_addr);
     try now exists cstate;
@@ -1168,11 +1091,13 @@ Proof.
     clear deployed_state deployed.
     apply wc_receive_strong in receive_some as
       (prev_state' & msg' & new_state' & serialize_prev_state & serialize_msg & serialize_new_state & receive_some).
-    setoid_rewrite deserialize_serialize in serialize_prev_state. inversion serialize_prev_state. subst.
+    setoid_rewrite deserialize_serialize in serialize_prev_state.
+    inversion serialize_prev_state. subst.
+    clear serialize_prev_state.
     apply receive_total_supply_increasing in receive_some as total_supply_increasing; try (cbn; lia).
     apply receive_preserves_constants in receive_some as (? & ? & ? & ? & ? & ? & ? & ?).
     repeat match goal with
-    | H : _ prev_state' =  _ new_state' |- _=> rewrite H in *; clear H
+    | H : _ prev_state' =  _ new_state' |- _=> try rewrite H in *; clear H
     end.
     eexists new_state'.
     repeat split; eauto;
@@ -1223,8 +1148,8 @@ Proof.
     induction accounts; intros.
     + (* If the queue is empty then we know that the funding goal was hit
           and can then apply can_finalize_if_creation_min *)
-      clear accounts_unique accounts_not_contracts finalized
-            funding_period_not_over funding_period_started.
+      clear accounts_unique accounts_not_contracts can_hit_fund_min echange_rate_nonzero
+            finalized funding_period_not_over funding_period_started.
       apply N.le_0_r, N.sub_0_le in enough_balance_to_fund.
       specialize (can_finalize_if_creation_min bstate0 reward caddr creator).
       intros []; eauto.
@@ -1233,7 +1158,6 @@ Proof.
     + clear reward Hreward creator Hcreator.
       apply NoDup_cons_iff in accounts_unique as [accounts_unique accounts_unique'].
       apply list.Forall_cons in accounts_not_contracts as [accounts_not_contracts accounts_not_contracts'].
-      apply not_in_cons in bat_fund_not_in_accounts as [bat_fund_not_in_accounts bat_fund_not_in_accounts'].
 
       (* Check if funding goal was alredy hit *)
       destruct (tokenCreationMin cstate - total_supply cstate) eqn:tokens_left_to_fund.
@@ -1282,16 +1206,8 @@ Proof.
               lia.
         }
 
-        specialize deployed_implies_constants_valid as
-            (cstate' & contract_state' & _ & _ & _ & echange_rate_nonzero & can_hit_fund_min); eauto.
-        cbn in contract_state'.
-        rewrite contract_state in contract_state'.
-        setoid_rewrite deserialize_serialize in contract_state'.
-        inversion contract_state'. subst cstate'.
-        clear contract_state'.
-
         (* Now we know that the action is valid we need to evaluate it *)
-        evaluate_action BATFixed.contract; try easy;
+        evaluate_action BAT.contract; try easy;
           only 1-4: clear fund_deposit_not_contract accounts_not_contracts IHaccounts.
         -- (* Prove that there is an action in the queue *)
            now rewrite create_token_acts_cons by lia.
@@ -1301,7 +1217,7 @@ Proof.
            nia.
         -- (* Prove that receive returns Some *)
            clear dependent accounts.
-           clear contract_state.
+           clear contract_deployed contract_state.
            apply Nat.ltb_ge in funding_period_started.
            apply Nat.ltb_ge in funding_period_not_over.
            cbn.
@@ -1309,7 +1225,6 @@ Proof.
              try (apply Z.ge_le, account_balance_nonnegative; eauto).
            clear finalized funding_period_started funding_period_not_over.
            cbn.
-           destruct_match eqn:match_sender; destruct_throw_if match_sender.
            destruct_match eqn:match_amount; destruct_throw_if match_amount.
            destruct_match eqn:match_cap; destruct_throw_if match_cap; eauto.
          --- (* Prove contradiction between match_amount, match_cap and can_hit_fund_min *)
@@ -1329,18 +1244,16 @@ Proof.
           ---- rewrite <- N2Z.inj_0 in min_left.
                now apply N2Z.inj_le, N_le_add_distr in min_left.
           ---- lia.
-         --- (* Prove contradiction between match_sender, bat_fund_not_in_accounts *)
-             now destruct_address_eq.
         -- assert (caddr_not_in_accounts : ~ In caddr accounts) by
              (intro; rewrite Forall_forall in accounts_not_contracts'; apply accounts_not_contracts' in H; now apply contract_addr_format in contract_deployed).
            (* Apply induction hypothesis *)
            edestruct IHaccounts as (bstate_new & reach_new & emptyable_new & H);
-             clear IHaccounts accounts_not_contracts balance_positive queue0 tokens_left_to_fund p can_hit_fund_min;
-             only 11: (rewrite deployed_state; eauto);
+             clear IHaccounts accounts_not_contracts balance_positive queue0 tokens_left_to_fund p;
+             only 12: (rewrite deployed_state; eauto);
              try (rewrite_environment_equiv; eauto);
              cbn; try rewrite Z2N.inj_min, N2Z.id;
              clear deployed_state contract_deployed funding_period_started funding_period_not_over
-                   fund_deposit_not_contract finalized contract_state.
+             can_hit_fund_min fund_deposit_not_contract finalized contract_state.
          --- (* Prove that the queues of the two ChainStates are equivalent *)
              rewrite queue, N.sub_add_distr.
              apply create_token_acts_eq.
@@ -1382,15 +1295,11 @@ Lemma can_deploy_and_finalize : forall bstate (reward : Amount) (caddr creator :
   (S (current_slot (env_chain bstate)) < (_fundingStart setup))%nat ->
   address_is_contract (_fundDeposit setup) = false ->
   setup.(_tokenExchangeRate) <> 0 ->
-  setup.(_batFund) <= setup.(_tokenCreationCap) ->
-  ~ In setup.(_batFundDeposit) accounts ->
-  setup.(_batFundDeposit) <> caddr ->
-  setup.(_fundDeposit) <> caddr ->
   exists bstate',
     reachable_through bstate bstate'
     /\ emptyable (chain_state_queue bstate')
     /\ exists cstate,
-    env_contracts bstate' caddr = Some (BATFixed.contract : WeakContract)
+    env_contracts bstate' caddr = Some (BAT.contract : WeakContract)
     /\ env_contract_states bstate' caddr = Some (serializeState cstate)
     /\ (isFinalized cstate) = true.
 Proof.
@@ -1406,13 +1315,9 @@ Proof.
          funding_period_nonempty
          funding_period_not_started
          fund_deposit_not_contract
-         echange_rate_nonzero
-         init_supply_le_cap
-         batfund_not_in_accounts
-         batfund_not_caddr
-         ethfund_not_caddr.
+         echange_rate_nonzero.
 
-  add_block [(deploy_act setup BATFixed.contract creator)] 1%nat; eauto. apply list.Forall_singleton, address_eq_refl.
+  add_block [(deploy_act setup BAT.contract creator)] 1%nat; eauto. apply list.Forall_singleton, address_eq_refl.
   update ((current_slot bstate0) < _fundingStart setup)%nat in funding_period_not_started by
     (rewrite_environment_equiv; cbn; lia).
   update bstate with bstate0 in enough_balance_to_fund by
@@ -1421,24 +1326,8 @@ Proof.
      intros; rewrite_environment_equiv; cbn; destruct_address_eq; try lia).
   update_all.
 
-  deploy_contract BATFixed.contract; eauto; try lia;
-    try now apply account_balance_nonnegative.
-  { (* Prove that init returns some *)
-    cbn.
-    destruct_match eqn:requirements; eauto.
-    destruct_throw_if requirements.
-    repeat apply Bool.orb_prop in requirements as [requirements | requirements].
-    - now apply Nat.leb_le in requirements.
-    - now apply Nat.ltb_lt in requirements.
-    - now apply N.ltb_lt in requirements.
-    - now apply N.ltb_lt in requirements.
-    - now apply N.eqb_eq in requirements.
-    - now apply N.ltb_lt in requirements.
-    - now destruct_address_eq.
-    - now destruct_address_eq.
-  }
-  specialize constants_are_constant as
-    (dep_info & cstate' & deploy_info' & deployed_state' & ? & ? & ? & ? & ? & ? & ? & ?); eauto.
+  deploy_contract BAT.contract; eauto; try lia; try now apply account_balance_nonnegative.
+  specialize constants_are_constant as (dep_info & cstate' & deploy_info' & deployed_state' & ? & ? & ? & ? & ? & ? & ? & ?); eauto.
   unfold contract_state in deployed_state'. cbn in deployed_state'.
   rewrite deployed_state, deserialize_serialize in deployed_state'.
   inversion deployed_state'. subst cstate'. clear deployed_state'.
@@ -1473,592 +1362,51 @@ Qed.
 
 
 
-(** ** BAToken outgoing acts facts *)
+(** ** Refund guarantee *)
 
-(** BAToken never calls itself *)
-Lemma bat_no_self_calls bstate caddr :
+(** The BAToken contract should guarantee that all tokens (except for the free initSupply given to batFundDeposit)
+    can be fully refunded. However as shown in the property based tests this is not the case so we can only prove
+    a weaker result stating that refund msgs can always be consumed. This does not guarantee refunding as the
+    proof does not state that the new actions produced by refund entrypoint can be evaluated. Thus it is not
+    guaranteed that the state changes will be applied *)
+Lemma weak_refund_guarantee : forall bstate cstate caddr account acts,
+  let refund_act := build_act account account (act_call caddr 0 refund) in
   reachable bstate ->
-  env_contracts bstate caddr = Some (contract : WeakContract) ->
-  Forall (fun act_body =>
-    match act_body with
-    | act_transfer to _ => (to =? caddr)%address = false
-    | _ => False
-    end) (outgoing_acts bstate caddr).
+  env_contracts bstate caddr = Some (BAT.contract : WeakContract) ->
+  env_contract_states bstate caddr = Some (serialize cstate) ->
+  chain_state_queue bstate = refund_act :: acts ->
+  (fundingEnd cstate < current_slot bstate)%nat -> (* funding period is over *)
+  total_supply cstate < tokenCreationMin cstate -> (* funding failed *)
+  account <> batFundDeposit cstate -> (* sender is not batFundDeposit *)
+  0 < with_default 0 (FMap.find account (balances cstate)) -> (* account owns some tokens *)
+  exists new_bstate new_acts, chain_state_queue new_bstate = new_acts ++ acts /\ inhabited (ActionEvaluation bstate refund_act new_bstate new_acts).
 Proof.
-  contract_induction; intros; auto.
-  - now inversion IH.
-  - apply Forall_app; split; auto.
-    clear IH.
-    instantiate (CallFacts := fun _ ctx state _ => fundDeposit state <> ctx_contract_address ctx).
-    destruct_message;
-      try now erewrite eip20_new_acts_correct by eauto.
-    + now contract_simpl.
-    + contract_simpl.
-      constructor; auto.
-      now destruct_address_eq.
-    + contract_simpl.
-      constructor; auto.
-      now destruct_address_eq.
-  - inversion_clear IH as [|? ? head_not_me tail_not_me].
-    apply Forall_app; split; auto.
-    clear tail_not_me.
-    destruct head; try contradiction.
-    destruct action_facts as [? _].
-    now destruct_address_eq.
-  - now rewrite <- perm.
-  - instantiate (DeployFacts := fun _ _ => True).
-    instantiate (AddBlockFacts := fun _ _ _ _ _ _ => True).
-    unset_all; subst.
-    destruct_chain_step; auto.
-    destruct_action_eval; auto.
-    intros ? contract_deployed ?.
-    cbn.
-    apply deployed_implies_constants_valid in contract_deployed; auto.
-    now destruct_hyps.
-Qed.
-
-Lemma bat_no_self_calls' : forall bstate origin from_addr to_addr amount msg acts,
-  reachable bstate ->
-  env_contracts bstate to_addr = Some (contract : WeakContract) ->
-  chain_state_queue bstate = {|
-    act_origin := origin;
-    act_from := from_addr;
-    act_body :=
-      match msg with
-      | Some msg => act_call to_addr amount msg
-      | None => act_transfer to_addr amount
-      end
-  |} :: acts ->
-  from_addr <> to_addr.
-Proof.
-  intros * reach deployed queue.
-  apply bat_no_self_calls in deployed as no_self_calls; auto.
-  unfold outgoing_acts in no_self_calls.
-  rewrite queue in no_self_calls.
-  cbn in no_self_calls.
-  destruct_address_eq; auto.
-  inversion_clear no_self_calls as [|? ? hd _].
-  destruct msg.
-  * congruence.
-  * now rewrite address_eq_refl in hd.
-Qed.
-
-(** BAToken only produces transfer acts *)
-Lemma outgoing_acts_are_transfers : forall bstate caddr,
-  reachable bstate ->
-  env_contracts bstate caddr = Some (contract : WeakContract) ->
-  Forall (fun act_body =>
-    match act_body with
-    | act_transfer _ _ => True
-    | _ => False
-    end) (outgoing_acts bstate caddr).
-Proof.
-  intros * reach deployed.
-  apply (lift_outgoing_acts_prop contract); auto.
-  intros * receive_some.
-  destruct_message;
-    (* m = EIP msg *)
-    try now erewrite eip20_new_acts_correct.
-  - (* m = create_tokens *)
-    now erewrite try_create_tokens_acts_correct.
-  - (* m = finalize *)
-    now erewrite try_finalize_acts_correct.
-  - (* m = refund *)
-    now erewrite try_refund_acts_correct.
-Qed.
-
-(** BAToken only produces transfer acts *)
-Lemma outgoing_acts_positive_amount : forall bstate caddr,
-  reachable bstate ->
-  env_contracts bstate caddr = Some (contract : WeakContract) ->
-  Forall (fun act_body => 0 <= act_body_amount act_body)%Z (outgoing_acts bstate caddr).
-Proof.
-  contract_induction; intros; auto.
-  - now inversion IH.
-  - instantiate (CallFacts := fun _ ctx _ _ =>
-      (0 <= (ctx_contract_balance ctx))%Z /\
-      ctx_from ctx <> ctx_contract_address ctx).
-    destruct facts as (contract_balance_positive & _).
-    destruct_message;
-      (* m = EIP msg *)
-      try now (apply eip20_new_acts_correct in receive_some; subst).
-    + (* m = create_tokens *)
-      apply try_create_tokens_acts_correct in receive_some.
-      now subst.
-    + (* m = finalize *)
-      apply try_finalize_acts_correct in receive_some.
-      subst.
-      now constructor.
-    + (* m = refund *)
-      apply try_refund_acts_correct in receive_some.
-      subst.
-      constructor; auto.
-      apply N2Z.is_nonneg.
-  - now destruct facts.
-  - eapply forall_respects_permutation; eauto.
-  - instantiate (AddBlockFacts := fun _ _ _ _ _ _ => True).
-    instantiate (DeployFacts := fun _ _ => True).
-    unset_all; subst.
-    destruct_chain_step; auto.
-    destruct_action_eval; auto.
-    intros cstate contract_deployed _. cbn.
-    subst. cbn.
-    split.
-    + (* Prove call fact: 0 <= ctx_contract_balance ctx *)
-      destruct_address_eq; subst; try easy.
-      * lia.
-      * apply Z.add_nonneg_nonneg; try lia.
-        now apply Z.ge_le, account_balance_nonnegative.
-    + (* Prove call fact: ctx_from ctx <> ctx_contract_address ctx *)
-      now eapply bat_no_self_calls'.
-Qed.
-
-
-
-(** ** batFundDeposit cannot refund *)
-
-(** batFundDeposit starts with initSupply tokens and should not be allowed
-    to refund them. Therefore if the token is not finalized then the
-    token balance of batFundDeposit should be equal to initSupply *)
-Lemma no_init_supply_refund : forall bstate caddr,
-  reachable bstate ->
-  env_contracts bstate caddr = Some (contract : WeakContract) ->
-  exists cstate,
-    contract_state bstate caddr = Some cstate
-    /\ (isFinalized cstate = false ->
-        FMap.find cstate.(batFundDeposit) (balances cstate) = Some cstate.(initSupply)).
-Proof.
-  intros *.
-  apply (lift_contract_state_prop contract);
-    intros *; clear bstate caddr.
-  - intros init_some not_finalized.
-    contract_simpl. cbn.
-    apply FMap.find_add.
-  - intros IH receive_some not_finalized.
-    destruct msg. destruct m.
-    + apply eip_only_changes_token_state in receive_some as finalized_unchanged.
-      rewrite <- finalized_unchanged in not_finalized.
-      contract_simpl.
-      rename H into finalized.
-      now setoid_rewrite not_finalized in finalized.
-    + eapply try_create_tokens_preserves_other_balances in receive_some as balance_preserved.
-      apply try_create_tokens_only_change_token_state in receive_some as finalized_unchanged.
-      rewrite <- finalized_unchanged in *. cbn.
-      now rewrite <- balance_preserved.
-      specialize try_create_tokens_is_some as (_ & (_ & _ & _ & _ & _ & from_not_batfund)); eauto.
-    + now apply try_finalize_isFinalized_correct in receive_some.
-    + eapply try_refund_preserves_other_balances in receive_some as balance_preserved.
-      apply try_refund_only_change_token_state in receive_some as finalized_unchanged.
-      rewrite <- finalized_unchanged in *. cbn.
-      now rewrite <- balance_preserved.
-      specialize try_refund_is_some as (_ & (_ & _ & _ & _ & from_not_batfund & _)); eauto.
-    + now contract_simpl.
-Qed.
-
-
-
-(** ** Total balance lower bound *)
-
-(** The total supply should never go under the initial supply since
-    batFundDeposit is not allowed to refund the initial supply *)
-Lemma total_supply_lower_bound : forall bstate caddr,
-  reachable bstate ->
-  env_contracts bstate caddr = Some (contract : WeakContract) ->
-  exists cstate,
-    contract_state bstate caddr = Some cstate
-    /\ initSupply cstate <= total_supply cstate.
-Proof.
-  contract_induction; intros; auto.
-  - cbn in init_some.
-    now contract_simpl.
-  - instantiate (CallFacts := fun _ ctx state _ =>
-      total_supply state = sum_balances state /\
-      (isFinalized state = false -> FMap.find state.(batFundDeposit) (balances state) = Some state.(initSupply)) /\
-      ctx_from ctx <> ctx_contract_address ctx).
-    destruct facts as (sum_balances_eq_total_supply & no_init_supply_refund & _).
-    destruct_message;
-      try apply eip_only_changes_token_state in receive_some as init_supply_unchanged.
-    + apply try_transfer_preserves_total_supply in receive_some as supply_unchanged.
-      now rewrite <- supply_unchanged, <- init_supply_unchanged.
-    + apply try_transfer_from_preserves_total_supply in receive_some as supply_unchanged.
-      now rewrite <- supply_unchanged, <- init_supply_unchanged.
-    + apply try_approve_preserves_total_supply in receive_some as supply_unchanged.
-      now rewrite <- supply_unchanged, <- init_supply_unchanged.
-    + contract_simpl.
-      cbn.
-      rewrite N.add_comm.
-      now apply N_add_le.
-    + now contract_simpl.
-    + specialize try_refund_is_some as (_ & (_ & not_finalized & _ & _ & from_not_batfund & _)); eauto.
-      apply receive_preserves_constants in receive_some as constants_unchanged.
-      destruct constants_unchanged as (_ & _ & _ & _ & _ & _ & _ & init_supply_unchanged).
-      erewrite <- try_refund_total_supply_correct, <- init_supply_unchanged; eauto.
-      rewrite sum_balances_eq_total_supply in *.
-      apply N.le_trans with (m := with_default 0 (FMap.find prev_state.(batFundDeposit) (balances prev_state))).
-      * now rewrite no_init_supply_refund.
-      * now apply balance_le_sum_balances_ne.
-  - now destruct facts.
-  - instantiate (AddBlockFacts := fun _ _ _ _ _ _ => True).
-    instantiate (DeployFacts := fun _ _ => True).
-    unset_all; subst.
-    destruct_chain_step; auto.
-    destruct_action_eval; auto.
-    intros ? contract_deployed deployed_cstate.
-    subst. cbn.
-    repeat split.
-    + now apply sum_balances_eq_total_supply in contract_deployed as
-        (cstate' & deployed_state' & ?).
-    + apply no_init_supply_refund in contract_deployed as
-        (cstate' & deployed_cstate' & ?); auto.
-      rewrite deployed_cstate' in deployed_cstate.
-      inversion deployed_cstate.
-      now subst cstate'.
-    + now eapply bat_no_self_calls'.
-Qed.
-
-
-
-(** ** No outgoing acts produces while funding *)
-
-Lemma funding_period_no_acts : forall bstate caddr,
-  reachable bstate ->
-  env_contracts bstate caddr = Some (contract : WeakContract) ->
-  exists cstate,
-    contract_state bstate caddr = Some cstate
-    /\ (isFinalized cstate = false /\
-        ((current_slot bstate <= fundingEnd cstate)%nat \/ tokenCreationMin cstate <= total_supply cstate) ->
-        outgoing_acts bstate caddr = []).
-Proof.
-  contract_induction; intros; auto; try rename H into not_finalized.
-  - now specialize (IH not_finalized).
-  - destruct_message;
-      try (
-        apply eip_only_changes_token_state in receive_some as finalized_unchanged;
-        apply eip20_new_acts_correct in receive_some as no_new_acts).
-    + apply try_transfer_preserves_total_supply in receive_some as supply_unchanged.
-      rewrite <- supply_unchanged, <- finalized_unchanged in not_finalized.
-      now rewrite IH, no_new_acts.
-    + apply try_transfer_from_preserves_total_supply in receive_some as supply_unchanged.
-      rewrite <- supply_unchanged, <- finalized_unchanged in not_finalized.
-      now rewrite IH, no_new_acts.
-    + apply try_approve_preserves_total_supply in receive_some as supply_unchanged.
-      rewrite <- supply_unchanged, <- finalized_unchanged in not_finalized.
-      now rewrite IH, no_new_acts.
-    + apply try_create_tokens_only_change_token_state in receive_some as finalized_unchanged.
-      apply try_create_tokens_acts_correct in receive_some as no_new_acts.
-      specialize try_create_tokens_is_some as (_ & (_ & _ & _ & funding_active & _)); eauto.
-      rewrite <- finalized_unchanged in not_finalized.
-      destruct not_finalized as [not_finalized _].
-      rewrite no_new_acts, IH; auto.
-    + apply try_finalize_isFinalized_correct in receive_some as finalized.
-      now destruct not_finalized as [not_finalized _].
-    + apply try_refund_only_change_token_state in receive_some as finalized_unchanged.
-      apply try_refund_total_supply_correct in receive_some as new_supply.
-      specialize try_refund_is_some as
-        (_ & (_ & _ & funding_over%lt_not_le & goal_not_hit & _)); eauto.
-      destruct not_finalized as [_ [funding_not_over | goal_hit]].
-      * now rewrite <- finalized_unchanged in funding_not_over.
-      * rewrite <- new_supply, <- finalized_unchanged in goal_hit.
-        now cbn in goal_hit.
-  - now instantiate (CallFacts := fun _ ctx _ _ => ctx_from ctx <> ctx_contract_address ctx).
-  - apply IH in not_finalized. subst.
-    now apply Permutation.Permutation_nil in perm.
-  - instantiate (AddBlockFacts := fun _ _ _ _ _ _ => True).
-    instantiate (DeployFacts := fun _ _ => True).
-    unset_all; subst.
-    destruct_chain_step; auto.
-    destruct_action_eval; auto.
-    intros.
-    subst. cbn.
-    now eapply bat_no_self_calls'.
-Qed.
-
-
-
-(** ** Token balances divisible by exchange rate *)
-
-Lemma token_balances_divisible : forall bstate caddr,
-  reachable bstate ->
-  env_contracts bstate caddr = Some (contract : WeakContract) ->
-  exists cstate,
-    contract_state bstate caddr = Some cstate
-    /\ (forall addr, addr <> batFundDeposit cstate ->
-        isFinalized cstate = false ->
-        with_default 0 (FMap.find addr (balances cstate)) mod tokenExchangeRate cstate = 0).
-Proof.
-  contract_induction; intros; auto;
-    try rename H into addr_not_batfund;
-    try rename H0 into not_finalized.
-  - cbn in init_some.
-    destruct_match in init_some; try congruence.
-    inversion init_some. subst. cbn in *.
-    setoid_rewrite FMap.find_add_ne; auto.
-  - instantiate (CallFacts := fun _ ctx state _ =>
-      tokenExchangeRate state <> 0 /\
-      ctx_from ctx <> ctx_contract_address ctx).
-    destruct facts as (exchange_rate_nonzero & _).
-    destruct msg. destruct m.
-    + apply eip_only_changes_token_state in receive_some as finalize_unchanged.
-      rewrite <- finalize_unchanged in not_finalized.
-      contract_simpl.
-      rename H into finalized.
-      now setoid_rewrite not_finalized in finalized.
-    + eapply try_create_tokens_only_change_token_state in receive_some as finalized_unchanged.
-      rewrite <- finalized_unchanged in *. cbn.
-      destruct (address_eqb addr (ctx_from ctx)) eqn:addr_from; destruct_address_eq; try easy.
-      * contract_simpl.
-        setoid_rewrite EIP20Token.add_is_partial_alter_plus; auto.
-        subst. clear addr_from.
-        setoid_rewrite FMap.find_add. cbn.
-        now rewrite N.add_mod, IH, N.add_mod_idemp_r, N.mod_add by assumption.
-      * erewrite <- try_create_tokens_preserves_other_balances; eauto.
-    + now apply try_finalize_isFinalized_correct in receive_some.
-    + eapply try_refund_only_change_token_state in receive_some as finalized_unchanged.
-      rewrite <- finalized_unchanged in *. cbn.
-      destruct (address_eqb addr (ctx_from ctx)) eqn:addr_from; destruct_address_eq; try easy.
-      * subst. clear addr_from.
-        erewrite try_refund_balance_correct; eauto.
-      * erewrite <- try_refund_preserves_other_balances; eauto.
-    + now contract_simpl.
-  - now destruct facts.
-  - instantiate (AddBlockFacts := fun _ _ _ _ _ _ => True).
-    instantiate (DeployFacts := fun _ _ => True).
-    unset_all; subst.
-    destruct_chain_step; auto.
-    destruct_action_eval; auto.
-    intros ? contract_deployed ?.
-    subst. cbn.
-    split.
-    * now specialize deployed_implies_constants_valid as
-        (cstate' & deployed_state' & _ & _ & _ & exchange_rate_nonzero & _).
-    * now eapply bat_no_self_calls'.
-Qed.
-
-
-
-(** **  Contract balance bound *)
-
-Lemma contract_balance_bound : forall bstate caddr (trace : ChainTrace empty_state bstate),
-  let effective_balance := (env_account_balances bstate caddr - (sumZ (fun act => act_body_amount act) (outgoing_acts bstate caddr)))%Z in
-  env_contracts bstate caddr = Some (contract : WeakContract) ->
-  exists cstate deploy_info,
-    contract_state bstate caddr = Some cstate
-    /\ deployment_info Setup trace caddr = Some deploy_info
-    /\ (isFinalized cstate = true -> effective_balance = 0)%Z
-    /\ (isFinalized cstate = false ->
-      (effective_balance - deploy_info.(deployment_amount)) * (Z.of_N cstate.(tokenExchangeRate)) =
-      (Z.of_N ((total_supply cstate) - cstate.(initSupply))))%Z.
-Proof.
-  intros *.
-  unfold effective_balance.
-  contract_induction; intros; auto; try destruct IH as [IH_finalized IH_funding].
-  - cbn in *.
-    destruct_match in init_some; try congruence.
-    inversion init_some. cbn.
-    split; intros.
-    + discriminate.
-    + lia.
-  - cbn in *.
-    split; intros.
-    + now rewrite <- IH_finalized by assumption.
-    + now rewrite <- IH_funding by assumption.
-  - instantiate (CallFacts := fun chain ctx state out_acts =>
-      (0 <= ctx_amount ctx)%Z /\
-      initSupply state <= total_supply state /\
-      tokenExchangeRate state <> 0 /\
-      (isFinalized state = false -> ctx_from ctx <> batFundDeposit state ->
-        N.modulo (with_default 0 (FMap.find ctx.(ctx_from) (balances state))) state.(tokenExchangeRate) = 0) /\
-      (isFinalized state = false -> ctx_from ctx <> batFundDeposit state ->
-        (with_default 0 (FMap.find ctx.(ctx_from) (balances state))) <= total_supply state - initSupply state) /\
-      (isFinalized state = false /\
-                    ((current_slot chain <= fundingEnd state)%nat \/
-                    tokenCreationMin state <= total_supply state) -> out_acts = []) /\
-      ctx_from ctx <> ctx_contract_address ctx).
-    destruct facts as (ctx_amount_positive &
-                       supply_bound &
-                       exchange_rate_nonzero &
-                       tokens_modulo_exchange_rate &
-                       tokens_bound &
-                       funding_no_outgoing_acts &
-                       _).
-    clear CallFacts AddBlockFacts DeployFacts.
-    destruct msg. destruct m.
-    + apply eip_only_changes_token_state in receive_some as finalized_unchanged.
-      apply eip20_new_acts_correct in receive_some as no_new_acts.
-      apply eip20_not_payable in receive_some as not_payable.
-      apply Z.le_antisymm in ctx_amount_positive; auto.
-      rewrite ctx_amount_positive, Z.sub_0_r in IH_finalized, IH_funding.
-      destruct m.
-      * apply try_transfer_preserves_total_supply in receive_some as supply_unchanged.
-        now rewrite no_new_acts, <- supply_unchanged, <- finalized_unchanged.
-      * apply try_transfer_from_preserves_total_supply in receive_some as supply_unchanged.
-        now rewrite no_new_acts, <- supply_unchanged, <- finalized_unchanged.
-      * apply try_approve_preserves_total_supply in receive_some as supply_unchanged.
-        now rewrite no_new_acts, <- supply_unchanged, <- finalized_unchanged.
-    + apply try_create_tokens_amount_correct in receive_some as payable.
-      contract_simpl.
-      subst. cbn in *.
-      rename H into requirements_check.
-      rewrite !Bool.orb_false_iff in requirements_check.
-      destruct requirements_check as (((not_finalized & _) & _) & _).
-      split; intros finalized_state.
-      * congruence.
-      * apply IH_funding in finalized_state.
-        rewrite N.add_sub_swap, N2Z.inj_add by assumption.
-        lia.
-    + contract_simpl.
-      subst. cbn in *.
-      rename H into not_payable.
-      rewrite Z.gtb_ltb, Z.ltb_ge in not_payable.
-      apply Z.le_antisymm in ctx_amount_positive; auto.
-      rewrite ctx_amount_positive, Z.sub_0_r in IH_finalized, IH_funding.
-      split; intros finalized_state.
-      * rewrite Z.sub_add_distr, Z.sub_diag, Z.sub_0_l, <- Z.opp_0, Z.opp_inj_wd.
-        rename H0 into requirements_check.
-        rewrite !Bool.orb_false_iff in requirements_check.
-        destruct requirements_check as ((not_finalized & _) & funding_hit%N.ltb_ge).
-        now rewrite funding_no_outgoing_acts.
-      * congruence.
-    + contract_simpl.
-      subst. cbn in *.
-      rename H into not_payable.
-      rewrite Z.gtb_ltb, Z.ltb_ge in not_payable.
-      apply Z.le_antisymm in ctx_amount_positive; auto.
-      rewrite ctx_amount_positive, Z.sub_0_r in IH_finalized, IH_funding.
-      rename H0 into requirements_check.
-      rename H1 into from_ne_batfund.
-      rename H2 into from_balance.
-      rewrite !Bool.orb_false_iff in requirements_check.
-      destruct requirements_check as ((finalized_sate & _) & _).
-      split; intros finalized_state.
-      * congruence.
-      * apply IH_funding in finalized_state.
-        update (ctx_from ctx <> batFundDeposit prev_state) in from_ne_batfund by now destruct_address_eq.
-        rewrite <- Z.sub_add_distr, (Z.add_comm _ (sumZ _ _)), Z.add_comm,
-                !Z.sub_add_distr, Z.mul_sub_distr_r, <- N2Z.inj_mul.
-        rewrite from_balance in tokens_bound.
-        apply tokens_bound in from_ne_batfund as tokens_bound'; auto.
-        apply tokens_modulo_exchange_rate in from_ne_batfund as tokens_modulo_exchange_rate'; auto.
-        rewrite <- N.div_exact, N.mul_comm, from_balance in tokens_modulo_exchange_rate' by auto.
-        setoid_rewrite <- tokens_modulo_exchange_rate'.
-        cbn in *.
-        lia.
-    + now contract_simpl.
-  - now destruct facts as (_ & _ & _ & _ & _ & no_self_calls).
-  - now erewrite sumZ_permutation in IH_finalized, IH_funding by eauto.
-  - instantiate (AddBlockFacts := fun _ _ _ _ _ _ => True).
-    instantiate (DeployFacts := fun _ _ => True).
-    unset_all; subst.
-    destruct_chain_step; auto.
-    destruct_action_eval; auto.
-    intros cstate contract_deployed deployed_cstate.
-    subst. cbn.
-    repeat split.
-    + now apply Z.ge_le.
-    + now apply total_supply_lower_bound in contract_deployed as
-        (cstate' & deployed_state' & ?).
-    + now apply deployed_implies_constants_valid in contract_deployed as
-      (cstate' & deployed_state' & _ & _ & _ & exchange_rate_nonzero & _).
-    + intros not_finalized from_not_batfund.
-      specialize token_balances_divisible as (cstate' & deployed_cstate' & ?); eauto.
-      rewrite deployed_cstate in deployed_cstate'.
-      inversion deployed_cstate'.
-      now subst cstate'.
-    + intros not_finalized from_not_batfund.
-      specialize no_init_supply_refund as (cstate' & deployed_cstate' & batfund_balance); eauto.
-      rewrite deployed_cstate in deployed_cstate'.
-      inversion deployed_cstate'.
-      subst cstate'. clear deployed_cstate'.
-      specialize sum_balances_eq_total_supply as (cstate' & deployed_cstate' & sum_eq_total); eauto.
-      rewrite deployed_cstate in deployed_cstate'.
-      inversion deployed_cstate'.
-      subst cstate'. clear deployed_cstate'.
-      replace (initSupply cstate) with (with_default 0 (FMap.find (batFundDeposit cstate) (balances cstate))) by
-        now rewrite batfund_balance.
-      rewrite sum_eq_total.
-      now apply balance_le_sum_balances_ne.
-    + intros.
-      specialize funding_period_no_acts as (cstate' & deployed_state' & no_acts); eauto.
-      now apply no_acts.
-    + now eapply bat_no_self_calls'.
-Qed.
-
-
-
-(** ** outgoing acts are valid *)
-
-(** Prove that all outgoing acts produced by the contract can be evaluated *)
-Lemma outgoing_acts_evaluable : forall bstate caddr,
-  reachable bstate ->
-  env_contracts bstate caddr = Some (contract : WeakContract) ->
-  Forall (fun act_body => receiver_can_receive_transfer bstate act_body) (outgoing_acts bstate caddr) ->
-  Forall (fun act_body => forall origin, exists bstate_new, inhabited (ActionEvaluation bstate (build_act origin caddr act_body) bstate_new [])) (outgoing_acts bstate caddr).
-Proof.
-  intros * reach deployed can_receive_funds.
-  assert (trace := reach).
-  destruct trace as [trace].
-  specialize contract_balance_bound as
-    (cstate & dep_info & deployed_state & deployed_info &
-    contract_balance_bound_finalized & contract_balance_bound); eauto.
-  apply deployment_amount_nonnegative in deployed_info as dep_amount_nonnegative.
-  specialize deployed_implies_constants_valid as
-    (cstate' & deployed_state' & _ & _ & _ & exchange_rate_nonzero & _); eauto.
-  rewrite deployed_state in deployed_state'.
+  intros * reach deployed deployed_state queue funding_over funding_failed account_not_batfund has_tokens.
+  subst refund_act.
+  eapply no_finalization_before_goal in reach as not_finalized; eauto.
+  destruct not_finalized as (cstate' & deployed_state' & not_finalized).
+  cbn in deployed_state'.
+  rewrite deployed_state, deserialize_serialize in deployed_state'.
   inversion deployed_state'.
   subst cstate'. clear deployed_state'.
-  eapply outgoing_acts_are_transfers in reach as acts_are_transfers; eauto.
-  eapply outgoing_acts_positive_amount in reach as acts_amount_positive; eauto.
-  apply Forall_forall.
-  intros act HIn.
-  eapply Forall_forall in acts_are_transfers; eauto.
-  eapply Forall_forall in acts_amount_positive as act_amount_positive; eauto.
-  eapply Forall_forall in can_receive_funds; eauto.
-  destruct act; try now exfalso.
-  clear acts_are_transfers.
-  assert (enough_balance : (act_body_amount (act_transfer to amount) <= env_account_balances bstate caddr)%Z).
-  { destruct (isFinalized cstate).
-    - apply Zminus_eq in contract_balance_bound_finalized; auto.
-      rewrite contract_balance_bound_finalized.
-      apply sumZ_in_le; eauto.
-      now apply Forall_forall.
-    - apply Z_div_mult in contract_balance_bound; auto; try lia.
-      eapply Z.add_cancel_r in contract_balance_bound.
-      rewrite Z.sub_add, <- N2Z.inj_div in contract_balance_bound.
-      assert (H : (forall n m p, 0 <= p -> n - m = p -> m <= n)%Z).
-      { intros. subst p. now apply Z.le_0_sub. }
-      apply H in contract_balance_bound.
-      -- eapply Z.le_trans; try apply contract_balance_bound.
-         apply sumZ_in_le; eauto.
-         now apply Forall_forall.
-      -- apply Z.add_nonneg_nonneg; auto.
-         apply N2Z.is_nonneg.
-  }
-  intros origin.
-  destruct can_receive_funds as [receive_not_contract | (wc & cstate' & deployed' & deployed_state' & new_state & receive_some )].
-  - eexists.
-    constructor.
-    eapply eval_transfer; auto.
-    + now apply Z.le_ge.
-    + now replace amount with (act_body_amount (act_transfer to amount)); auto.
-    + assumption.
+  eexists {| chain_state_env := _; chain_state_queue := _ |}.
+  eexists.
+  split; cycle 1.
+  - constructor.
+    eapply eval_call with (msg := Some _); eauto.
+    + lia.
+    + now apply Z.ge_le, account_balance_nonnegative.
+    + specialize try_refund_is_some as [[new_cstate [resp_acts receive_some]] _]; cycle 1.
+      * apply wc_receive_to_receive.
+        rewrite receive_some.
+        contract_simpl.
+        rename H1 into account_balance_some.
+        replace n with (with_default 0 (FMap.find account (balances cstate))); auto.
+        now rewrite account_balance_some.
+      * repeat split; eauto.
     + now constructor.
-  - eexists.
-    constructor.
-    eapply eval_call with (msg := None); eauto; cycle -1.
-    + now constructor.
-    + apply Z.le_ge.
-      apply act_amount_positive.
-    + cbn.
-      replace (env_account_balances (set_contract_state to new_state (transfer_balance caddr to amount bstate)) to)
-        with (((env_account_balances bstate to) + amount)%Z).
-      * apply receive_some.
-      * apply bat_no_self_calls in deployed; auto.
-        eapply Forall_forall in deployed; eauto.
-        cbn in *.
-        destruct_address_eq; easy.
-    + eauto.
-  Unshelve. auto.
+  - eauto.
 Qed.
 
 End Theories.
-End BATFixed.
+End BAT.
