examples/bat/BATPrinters.v
@@ -1,11 +1,10 @@
 From ConCert.Execution Require Import Blockchain.
 From ConCert.Execution Require Import Serializable.
-From ConCert.Execution.Examples Require Import BATCommon.
-From ConCert.Execution.QCTests Require Import EIP20TokenPrinters.
+From ConCert.Examples.BAT Require Import BATCommon.
+From ConCert.Examples.EIP20 Require Import EIP20TokenPrinters.
 From ConCert.Execution.QCTests Require Import TestUtils.
 From ConCert.Execution.QCTests Require Import SerializablePrinters.
 From QuickChick Require Import QuickChick.
-
 
 Local Open Scope string_scope.
 
