examples/bat/BATTestCommon.v
@@ -6,9 +6,9 @@ From ConCert.Execution Require Import Extras.
 From ConCert.Execution Require Import Containers.
 From ConCert.Execution Require Import LocalBlockchain.
 From ConCert.Execution Require Import Serializable.
-From ConCert.Execution.Examples Require Import BATCommon.
-From ConCert.Execution.QCTests Require Import BATGens.
-From ConCert.Execution.QCTests Require Import BATPrinters.
+From ConCert.Examples.BAT Require Import BATCommon.
+From ConCert.Examples.BAT Require Import BATGens.
+From ConCert.Examples.BAT Require Import BATPrinters.
 From ConCert.Execution.QCTests Require Import ChainPrinters.
 From ConCert.Execution.QCTests Require Import SerializablePrinters.
 From ConCert.Execution.QCTests Require Import TestUtils.
