examples/bat/BAT_AltFix.v
@@ -21,9 +21,9 @@ From ConCert.Execution Require Import Containers.
 From ConCert.Execution Require Import Extras.
 From ConCert.Execution Require Import Monads.
 From ConCert.Execution Require Import Serializable.
-From ConCert.Execution.Examples Require Import BATCommon.
-From ConCert.Execution.Examples Require Import Common.
-From ConCert.Execution.Examples Require EIP20Token.
+From ConCert.Execution Require Import Common.
+From ConCert.Examples.BAT Require Import BATCommon.
+From ConCert.Examples.EIP20 Require EIP20Token.
 Import RecordSetNotations.
 Import ListNotations.
 
